\section{Error Analysis}

    we know for \hyperref[tab:1]{Table 1} that:

    $$g = \frac{p\lambda}{\sin\theta} \;\;\;\;\;\;\;\;\;(p = 1\;and\;\Delta\lambda = 0)$$
    
    $$\therefore \Delta g = -p\lambda \cot\theta\;cosec\;\theta\;\Delta \theta$$
    $$\therefore \frac{\Delta g}{g} = - \cot\theta\Delta \theta$$


    $\therefore \Delta g = g \cot\theta\Delta \theta$ \hspace{2mm} [taking $\theta = 20.503^\circ$ (average $\theta$)]
    
    \hspace{3mm}
    $= 1.579\times 10^{-6} \times 2.674 \times 1.45 \times 10^{-4} = 6.1\times 10^{-10}$
    \begin{center}\fbox{$\therefore g = 1578.95\pm0.61\;nm$}\end{center}
    



    Differenciating \hyperref[eqn:2]{Eqn 2} we get:

    $$\Delta\lambda = g\cos\theta^{'}\Delta\theta^{'} + \sin\theta^{'}\Delta g$$
    $$\frac{\Delta\lambda}{\lambda} = \cot\theta^{'}\Delta\theta^{'} + \frac{\Delta g}{g}$$
    $$\frac{\Delta\lambda}{\lambda} =  (\cot\theta^{'}-\cot\theta)\Delta\theta$$

    taking $\theta^{'} = 20.835^\circ$ (average $\theta$),
    
    \hspace{1cm} $\Delta \theta = \Delta \theta^{'}= \frac{30}{60^2}^\circ = 1.45\times 10^{-4} rad$
    
    \hspace{1cm} $g = 1.579 \times 10^{-6}\;m$

    $$
    \frac{\Delta\lambda}{\lambda} = 6.74\times 10^{-6}
    $$

    Now differenciating \hyperref[eqn:1]{Eqn 1} we get:

    $$\frac{\Delta R_y}{R_y} = -\frac{\Delta \lambda}{\lambda} = 6.74\times 10^{-6}$$

    \begin{center}\fbox{$\therefore R_y = (1.0242 \times 10^{7} \pm 69)\;m^{-1}$}\end{center}

